increase instead of add, no more commutative

SlowTest/SMN-ADT-ListContLen-Inc.dfy
@@ -16,147 +16,102 @@ predicate AbPos (n: AbInt) { !AbIsZero(n) }
 // predicate AbNonNeg (n: AbInt) { true }
 
 function method AbLt(n: AbInt, m: AbInt) : bool
-function method AbAdd(n: AbInt, m: AbInt) : (r: AbInt)
-function method AbSub(n: AbInt, m: AbInt) : (r: AbInt)
+function method AbInc1(n: AbInt): (r: AbInt)
+function method AbInc(n: AbInt, m: AbInt) : (r: AbInt)
+function method AbDec(n: AbInt, m: AbInt) : (r: AbInt)
 function method AbDiv2(n: AbInt): (r: AbInt)
-  ensures AbLt(AbAdd(r, r), n) || AbAdd(r, r) == n
+  ensures AbLt(AbInc(r, r), n) || AbInc(r, r) == n
 function method AbSetLen(s: set<AbInt>) : (l: AbInt)
 lemma SetLen_Props()
   ensures forall x :: AbSetLen(x) == int2adt(0) <==> x == {}
   ensures forall x: AbInt :: AbSetLen({x}) == int2adt(1)
-  ensures forall x: AbInt, A: set<AbInt> :: x in A ==> AbSetLen(A) == AbAdd(AbSetLen(A - {x}), int2adt(1))
-  
-  // ensures forall x: AbInt, A, B: set<AbInt> :: x in A && x in B ==> 
-  // ensures forall A: set<AbInt>, B : set<AbInt> :: AbAdd(AbSetLen(A+B), AbSetLen(A*B)) == AbAdd(AbSetLen(A), AbSetLen(B))
-  // ensures forall A: set<AbInt>, B : set<AbInt> :: AbAdd(AbSetLen(A-B), AbSetLen(A*B)) == AbSetLen(A)
-  // ensures forall A: set<AbInt>, B : set<AbInt> :: A !! B ==> AbSetLen(A+B) == AbAdd(AbSetLen(A), AbSetLen(B))
-  // ensures forall A: set<AbInt>, B : set<AbInt> :: AbLt(AbSetLen(A+B), AbAdd(AbSetLen(A), AbSetLen(B))) || AbSetLen(A+B) == AbAdd(AbSetLen(A), AbSetLen(B))
+  ensures forall x: AbInt, A: set<AbInt> :: x in A ==> AbSetLen(A) == AbInc1(AbSetLen(A - {x}))
 
 // Set generation: lo <= x < lo+len
 // experiment with more trigger options
 function method AbBoundSet(lo: AbInt, len: AbInt): (S: set<AbInt>)
   ensures AbSetLen(S) == len
-  ensures forall x :: (AbLt(lo, x) || lo == x) && AbLt(x, AbAdd(lo, len)) <==> x in S
+  ensures forall x :: (AbLt(lo, x) || lo == x) && AbLt(x, AbInc(lo, len)) <==> x in S
   // Try not to assign every element with AbAdd()
   // ensures S == set x | 0 <= x < len :: AbAdd(lo, int2adt(x))
 
 /* Properties */
 lemma Props_int_pos(a: int)
   ensures AbPos(int2adt(a))
-lemma Props_int_cmp_lt(a: int, b: int) // Lt(a, b)
-  ensures AbLt(int2adt(a), int2adt(b))
-
-// lemma Props ()
-//   // Props_all_nonneg ()
-//   ensures forall x :: AbLt(int2adt(0), x) || x == int2adt(0)
-//   // Props_lt_is_not_geq ()
-//   ensures forall x, y :: AbLt(x, y) <==> !(AbLt(y, x) || x == y)
-//   // Props_lt_addition ()
-//   ensures forall x, a, b:: AbLt(a, b) ==> AbLt(AbAdd(x, a), AbAdd(x, b))
-//   // Props_lt_transitive ()
-//   ensures forall x, y, z :: AbLt(x, y) && AbLt(y, z) ==> AbLt(x, z)
-//   // Props_add_identity ()
-//   ensures forall x :: AbAdd(x, int2adt(0)) == AbAdd(int2adt(0), x) == x
-//   // Props_add_less_is_lt ()
-//   ensures forall x, y, a, b :: (x == AbAdd(y, a)) && AbLt(a, b) ==> AbLt(x, AbAdd(y, b))
-//   // Props_add_is_leq ()
-//   ensures forall x, y, a :: (AbAdd(x, a) == y) ==> AbLt(x, y) || x == y
-//   // Props_lt_add_is_lt ()
-//   ensures forall x, y, a :: AbLt(AbAdd(x, a), y) ==> AbLt(x, y)
-//   // Props_add_pos_is_neq ()
-//   ensures forall x, a :: AbPos(a) ==> AbAdd(x, a) != x
-//   // Props_one_in_bound ()
-//   ensures forall a, x :: (AbLt(a, x) || a == x) && (AbLt(x, AbAdd(a, int2adt(1)))) ==> a == x
-  // Props_add_sub_is_add ()
-  // ensures forall x: AbInt, i, j: int :: AbAdd(AbAdd(x, int2adt(j)), int2adt(i-j)) == AbAdd(x, int2adt(i)) // trigger may loop
-  // ensures forall x: AbInt, i, j, k: int :: k == i - j ==> AbAdd(AbAdd(x, int2adt(j)), int2adt(k)) == AbAdd(x, int2adt(i))
-
-// duplicate with Props ()
-// Note: if comment out, SMN_Correct doesn't finish.
 lemma Props_all_nonneg ()
   ensures forall x :: AbLt(int2adt(0), x) || x == int2adt(0)
 lemma Props_one_in_bound ()
-  ensures forall a, x :: (AbLt(a, x) || a == x) && (AbLt(x, AbAdd(a, int2adt(1)))) ==> a == x
-lemma Props_two_is_one_plus_one ()
-  ensures int2adt(2) == AbAdd(int2adt(1), int2adt(1))
-lemma Props_gtzero_is_geqone ()
-  ensures forall x :: AbLt(int2adt(0), x) <==> AbLt(int2adt(1), x) || x == int2adt(1)
-lemma Props_gtzero_is_geqone_param (x: AbInt)
-  ensures AbLt(int2adt(0), x) <==> AbLt(int2adt(1), x) || x == int2adt(1)
-
-lemma Props_lt_is_not_geq () // x < y <==> !x > y && x != y
+  ensures forall a, x :: (AbLt(a, x) || a == x) && (AbLt(x, AbInc1(a))) ==> a == x
+lemma Props_inc_one ()
+  ensures forall x :: AbInc1(x) == AbInc(x, int2adt(1)) == AbInc(int2adt(1), x)
+lemma Props_inc_zero ()
+  ensures forall x :: AbInc(x, int2adt(0)) == AbInc(int2adt(0), x) == x
+lemma Props_1inc1_is_2 ()
+  ensures AbInc1(int2adt(1)) == int2adt(2)
+lemma Props_lt2gteq () // x < y <==> !x > y && x != y
   ensures forall x, y :: AbLt(x, y) <==> !(AbLt(y, x) || x == y)
+lemma Props_inc2dec ()
+  ensures forall x, y, z :: AbInc(x, y) == z ==> AbDec(z, x) == y && AbDec(z, y) == x
+lemma Props_gt0_is_geq1 ()
+  ensures forall x :: AbLt(int2adt(0), x) <==> AbLt(int2adt(1), x) || x == int2adt(1)
+// lemma Props_gt0_is_geq1_param (x: AbInt)
+//   ensures AbLt(int2adt(0), x) <==> AbLt(int2adt(1), x) || x == int2adt(1)
+
 lemma Props_lt_addition () // a < b ==> x + a < x + b
-  ensures forall x, a, b:: AbLt(a, b) ==> AbLt(AbAdd(x, a), AbAdd(x, b))
+  ensures forall x, a, b:: AbLt(a, b) ==> AbLt(AbInc(x, a), AbInc(x, b))
 lemma Props_lt_transitive () // x < y < z
   ensures forall x, y, z :: AbLt(x, y) && AbLt(y, z) ==> AbLt(x, z)
-lemma Props_lt_add_is_lt () // x + a < y ==> x < y
-  ensures forall x, y, a :: AbLt(AbAdd(x, a), y) ==> AbLt(x, y)
+lemma Props_lt_inc_is_lt () // x + a < y ==> x < y
+  ensures forall x, y, a :: AbLt(AbInc(x, a), y) ==> AbLt(x, y)
 
-lemma Props_add_commutative () // x + y == y + x
-  ensures forall x, y :: AbAdd(x, y) == AbAdd(y, x);
-lemma Props_add_associative () // (x + y) + z == x + (y + z)
-  ensures forall x, y, z :: AbAdd(AbAdd(x, y), z) == AbAdd(x, AbAdd(y, z))
-lemma Props_add_addition () // x + a == y + a ==> x == y
-  ensures forall x, y, a :: AbAdd(x, a) == AbAdd(y, a) <==> x == y
-lemma Props_add_identity () // x + 0 == 0 + x == x
-  ensures forall x :: AbAdd(x, int2adt(0)) == AbAdd(int2adt(0), x) == x
-
-lemma Props_add_less_is_lt () // x = y + a && a < b ==> x < y + b
-  ensures forall x, y, a, b :: (x == AbAdd(y, a)) && AbLt(a, b) ==> AbLt(x, AbAdd(y, b))
+// lemma Props_inc_commutative () // x + y == y + x
+//   ensures forall x, y :: AbInc(x, y) == AbInc(y, x);
+lemma Props_inc_associative () // (x + y) + z == x + (y + z)
+  ensures forall x, y, z :: AbInc(AbInc(x, y), z) == AbInc(x, AbInc(y, z))
+lemma Props_inc_addition () // x + a == y + a ==> x == y
+  ensures forall x, y, a :: AbInc(x, a) == AbInc(y, a) <==> x == y
+lemma Props_inc_pos_is_pos () // x + Positive is Positive
+  ensures forall x, y :: AbPos(y) ==> AbPos(AbInc(x, y))
+  ensures forall x, y :: AbPos(y) ==> AbPos(AbInc(y, x))
+lemma Props_inc_pos_is_lt () // x < x + Positive
+  ensures forall x, y :: AbPos(y) ==> AbLt(x, AbInc(x, y))
+  ensures forall x, y :: AbPos(y) ==> AbLt(x, AbInc(y, x))
+lemma Props_inc_lt_is_lt () // x = y + a && a < b ==> x < y + b
+  ensures forall x, y, a, b :: (x == AbInc(y, a)) && AbLt(a, b) ==> AbLt(x, AbInc(y, b))
 // Some instantiation
-lemma Props_add_less_is_lt_param (x: AbInt, y: AbInt, a: AbInt, b: AbInt)
-  // Props_add_less_is_lt_param(s, n, int2adt(llen), int2adt(len));
-  ensures (x == AbAdd(y, a)) && AbLt(a, b) ==> AbLt(x, AbAdd(y, b))
+lemma Props_inc_lt_is_lt_param (x: AbInt, y: AbInt, a: AbInt, b: AbInt)
+  ensures (x == AbInc(y, a)) && AbLt(a, b) ==> AbLt(x, AbInc(y, b))
 
-lemma Props_add_is_leq () //  x + a == y ==> x < y || x == y
-  ensures forall x, y, a :: (AbAdd(x, a) == y) ==> AbLt(x, y) || x == y
-lemma Props_add_pos_is_neq () // x + Positive != x
-  ensures forall x, a :: AbPos(a) ==> AbAdd(x, a) != x
-lemma Props_add_pos_is_pos () // x + Positive is Positive
-  ensures forall x, a :: AbPos(a) ==> AbPos(AbAdd(x, a)) 
-lemma Props_add_pos_is_lt () // x < x + Positive
-  ensures forall x, a :: AbPos(a) ==> AbLt(x, AbAdd(x, a));
-lemma Props_add2sub () // x + y == z ==> x = z - y && y = z - x
-  ensures forall x, y, z :: AbAdd(x, y) == z ==> AbSub(z, y) == x && AbSub(z, x) == y
-
-lemma Props_add_sub_is_add () // x + j + (i - j) == x + i
-    ensures forall x, i, j :: AbAdd(AbAdd(x, j), AbSub(i, j)) == AbAdd(x, i) // trigger may loop
-    // ensures forall x: AbInt, i, j, k: int :: k == i - j ==> AbAdd(AbAdd(x, int2adt(j)), int2adt(k)) == AbAdd(x, int2adt(i))
+lemma Props_inc_dec_is_inc () // x + j + (i - j) == x + i
+    ensures forall x, i, j :: AbInc(AbInc(x, j), AbDec(i, j)) == AbInc(x, i) // trigger may loop
 // Some instantiation
-lemma Props_add_sub_is_add_param(x: AbInt, i: AbInt, j: AbInt)
-  // Props_add_sub_is_add_param(n, len, llen);
-  ensures AbAdd(AbAdd(x, j), AbSub(i, j)) == AbAdd(x, i)
+lemma Props_inc_dec_is_inc_param(x: AbInt, i: AbInt, j: AbInt)
+  ensures AbInc(AbInc(x, j), AbDec(i, j)) == AbInc(x, i)
 
-lemma Props_div_pos_is_pos () // Positive / 2 is Positive
-  ensures forall x :: AbPos(x) <==> AbPos(AbDiv2(x))
-lemma Props_div_add_leq_is_leq () // y <= x ==> (x+y)/2 <= x
-  ensures forall x, y :: AbLt(y, x) || x == y ==> AbLt(AbDiv2(AbAdd(x, y)), x) || AbDiv2(AbAdd(x, y)) == x
-lemma Props_div_add_leq_is_leq_param (x: AbInt, y: AbInt)
-  ensures AbLt(y, x) || x == y ==> AbLt(AbDiv2(AbAdd(x, y)), x) || AbDiv2(AbAdd(x, y)) == x
-lemma Props_div_addone_lt ()
-  ensures forall x :: AbLt(int2adt(1), x) || x == int2adt(1) ==> AbLt(AbAdd(AbDiv2(x), int2adt(1)), x)
-lemma Props_div_addone_lt_param (x: AbInt)
-  ensures AbLt(int2adt(1), x) || x == int2adt(1) ==> AbLt(AbAdd(AbDiv2(x), int2adt(1)), x)
-
-// lemma Props_unfold_int2adt (i: nat)
-//   ensures i == 0 ==> int2adt(i) == int2adt(0)
-//   ensures i != 0 ==> int2adt(i) == AbAdd(int2adt(1), int2adt(i-1))
+lemma Props_div_pos () // x > 1 ==> x/2 is Positive
+  ensures forall x :: AbLt(int2adt(1), x) ==> AbPos(AbDiv2(x))
+lemma Props_div_inc1_is_leq () // 1 <= x ==> (x+1)/2 <= x
+  ensures forall x :: AbLt(int2adt(1), x) || x == int2adt(1) ==> AbLt(AbDiv2(AbInc1(x)), x) || AbDiv2(AbInc1(x)) == x
+lemma Props_div_inc1_is_leq_param (x: AbInt)
+  ensures AbLt(int2adt(1), x) || x == int2adt(1) ==> AbLt(AbDiv2(AbInc1(x)), x) || AbDiv2(AbInc1(x)) == x
+lemma Props_div_and_inc1_is_leq () // 1 <= x ==> x/2+1 <= x
+  ensures forall x :: AbLt(int2adt(1), x) || x == int2adt(1) ==> AbLt(AbInc1(AbDiv2(x)), x) || AbInc1(AbDiv2(x)) == x
+lemma Props_div_and_inc1_is_leq_param (x: AbInt)
+  ensures AbLt(int2adt(1), x) || x == int2adt(1) ==> AbLt(AbInc1(AbDiv2(x)), x) || AbInc1(AbDiv2(x)) == x
 
 function method Length(xs: List<AbInt>): AbInt
 {
   match xs
   case Nil => int2adt(0)
-  case Cons(_, tail) =>  AbAdd(int2adt(1), Length(tail))
+  case Cons(_, tail) => AbInc1(Length(tail))
 }
  
 function method Split(xs: List<AbInt>, b: AbInt): (List<AbInt>, List<AbInt>)
-  ensures var r := Split(xs, b); Length(xs) == AbAdd(Length(r.0), Length(r.1))
+  ensures var r := Split(xs, b); Length(xs) == AbInc(Length(r.0), Length(r.1))
   decreases xs
 {
-  Props_add_commutative ();
-  Props_add_associative ();
-  Props_add_identity ();
+  Props_inc_associative ();
+  Props_inc_zero (); Props_inc_one ();  
   match xs
   case Nil => (Nil, Nil)
   case Cons(x, tail) =>
@@ -192,8 +147,8 @@ lemma Elements_Property(xs: List<AbInt>)
   ensures AbSetLen(Elements(xs)) == Length(xs)
 {
   SetLen_Props();
-  Props_add_commutative ();
-  Props_add_associative ();
+  // Props_add_commutative ();
+  Props_inc_associative ();
 }
 
 predicate NoDuplicates(xs: List<AbInt>)
@@ -212,9 +167,9 @@ lemma Cardinality(A: set<AbInt>, B: set<AbInt>)
 {
   SetLen_Props ();
   Props_all_nonneg ();
-  Props_add_addition ();
-  Props_add_commutative ();
+  Props_inc_addition ();
   Props_lt_addition ();
+  Props_inc_zero (); Props_inc_one ();
   if A != {} {
     var x :| x in A;
     Cardinality(A - {x}, B - {x});
@@ -226,7 +181,8 @@ lemma SetEquality(A: set<AbInt>, B: set<AbInt>)
   ensures A == B
 {
   SetLen_Props ();
-  Props_add_addition ();
+  Props_inc_addition ();
+  Props_inc_zero (); Props_inc_one ();
   if A == {} {
   } else {
     var x :| x in A;
@@ -238,10 +194,9 @@ function IntRange(lo: AbInt, len: AbInt): set<AbInt>
   ensures AbSetLen(IntRange(lo, len)) == len
 {
   var S := AbBoundSet(lo, len);
-  // assume AbLt(int2adt(len - 1), int2adt(len));
   // Try not to assign every element with AbAdd()
   // assert len != 0 ==> S == IntRange(lo, len - 1) + {AbAdd(lo, int2adt(len - 1))};
-  assert forall x :: ((AbLt(lo, x) || lo == x) && AbLt(x, AbAdd(lo, len))) ==> x in S;
+  assert forall x :: ((AbLt(lo, x) || lo == x) && AbLt(x, AbInc(lo, len))) ==> x in S;
   S
 }
 
@@ -254,26 +209,31 @@ function method SMN(xs: List<AbInt>, n: AbInt, len: AbInt): AbInt
   requires len == Length(xs)
   decreases adt2dt(len)
 {
-  Props_add_commutative ();
   if AbLt(int2adt(2), len) || int2adt(2) == len then
-    var (L, R) := Split(xs, AbAdd(n, AbDiv2(len)));
+    var (L, R) := Split(xs, AbInc(n, AbDiv2(len)));
     var llen := Length(L);
-    Props_all_nonneg ();
-    Props_lt_is_not_geq ();
-    Props_int_pos(2); // AbInt0 < AbInt2
-    Props_add_pos_is_lt ();
+
+    /* Props for ITE */
+    Props_lt_transitive (); // 0 < len
+    Props_lt2gteq ();
+
     if AbLt(llen, AbDiv2(len)) then
-      Props_lt_transitive (); // AbInt0 < len
-      Props_lt_add_is_lt ();
-      Props_adt_dt_lt (llen, len);
+      Props_int_pos(2); // 0 < 2
+      Props_lt_inc_is_lt (); // x + a < y ==> x < y
+      Props_adt_dt_lt (llen, len); // decreases (pre: llen < len/2 < len)
       SMN(L, n, llen)
     else
-      Props_div_pos_is_pos ();
-      Props_add2sub ();
-      Props_adt_dt_lt (AbSub(len, llen), len);
-      SMN(R, AbAdd(n, llen), AbSub(len, llen))
+      Props_all_nonneg ();
+      Props_int_pos(1);
+      Props_1inc1_is_2 ();
+      Props_inc_one (); // 1 < 2
+      Props_inc_pos_is_lt ();
+      Props_div_pos (); // 1 <= len/2
+      Props_inc2dec ();
+      Props_adt_dt_lt (AbDec(len, llen), len);
+      SMN(R, AbInc(n, llen), AbDec(len, llen))
   else if xs.Cons? then
-    if xs.head == n then AbAdd(n, int2adt(1)) else n
+    if xs.head == n then AbInc1(n) else n
   else
     n
 }
@@ -297,59 +257,68 @@ lemma SMN_Correct(xs: List<AbInt>, n: AbInt, len: AbInt)
   requires len == Length(xs)
   ensures var s := SMN(xs, n, len);
     (AbLt(n, s) || n == s) &&
-    (AbLt(s, AbAdd(n, len)) || s == AbAdd(n, len)) &&
+    (AbLt(s, AbInc(n, len)) || s == AbInc(n, len)) &&
     s !in Elements(xs) &&
-    forall x ::(AbLt(n, x) || n == x) && AbLt(x, s) ==> x in Elements(xs)
+    forall x :: (AbLt(n, x) || n == x) && AbLt(x, s) ==> x in Elements(xs)
   decreases adt2dt(len)
 {
-  Props_add_commutative (); // x + y = y + x
-  Props_all_nonneg ();
-  Props_lt_is_not_geq (); // x < y <==> !x > y && x != y
   if AbLt(int2adt(2), len) || int2adt(2) == len {
-    var (L, R) := Split(xs, AbAdd(n, AbDiv2(len)));
-    Split_Correct(xs, AbAdd(n, AbDiv2(len)));
+    var (L, R) := Split(xs, AbInc(n, AbDiv2(len)));
+    Split_Correct(xs, AbInc(n, AbDiv2(len)));
     var llen := Length(L);
     Elements_Property(L);  // NoDuplicates property
     var bound := IntRange(n, AbDiv2(len));
     Cardinality(Elements(L), bound);
-    Props_int_pos(2); // 0 < 2
-    Props_div_pos_is_pos ();
-    Props_add_pos_is_lt (); // x < x + Positive
-    Props_lt_add_is_lt (); // x + Postive < y ==> x < y
+
+    /* Props for ITE */
+    Props_lt_transitive (); // 0 < len
+    Props_lt2gteq ();
+
     if AbLt(llen, AbDiv2(len)) {
       var s := SMN(L, n, llen);
-      Props_lt_transitive (); // x < y < z      
-      Props_adt_dt_lt (llen, len); // decreases (pre: llen < len/2 < len)
+      Props_int_pos(2); // 0 < 2
+      Props_lt_inc_is_lt (); // x + a < y ==> x < y
+      Props_adt_dt_lt (llen, len);
       SMN_Correct(L, n, llen);
+
+      /* map boundary */
       Props_lt_addition (); // a < b ==> x + a < x + b: Lt(s, n+llen) ==> Lt(s, n+len)
-      // Props_add_less_is_lt ();  // x = y + a && a < b ==> x < y + b: s==n+llen ==> Lt(s, n+len)
-      Props_add_less_is_lt_param(s, n, llen, len); // no trigger loop
-    } else {
-      Props_add2sub ();
-      Props_adt_dt_lt (AbSub(len, llen), len);
-      var s := SMN(R, AbAdd(n, llen), AbSub(len, llen));
-      SMN_Correct(R, AbAdd(n, llen), AbSub(len, llen));
-      Props_add_is_leq (); // x + a == y ==> x < y || x == y: n+llen == s ==> Lt(n, s)
-      // Props_add_sub_is_add();
-      Props_add_sub_is_add_param(n, len, llen); // no trigger loop
+      // Props_inc_lt_is_lt (); // x = y + a && a < b ==> x < y + b: s==n+llen ==> Lt(s, n+len)
+      Props_inc_lt_is_lt_param(s, n, llen, len); // no trigger loop
+    }
+    
+    else {
+      Props_all_nonneg ();
+      Props_inc2dec ();
+      var s := SMN(R, AbInc(n, llen), AbDec(len, llen));
+      Props_int_pos(1);
+      Props_1inc1_is_2 ();
+      Props_inc_one (); // 1 < 2
+      Props_inc_pos_is_lt ();
+      Props_div_pos (); // 1 <= len/2
+      Props_adt_dt_lt (AbDec(len, llen), len);
+      SMN_Correct(R, AbInc(n, llen), AbDec(len, llen));
+
+      /* map boundary */
+      // Props_inc_dec_is_inc();
+      Props_inc_dec_is_inc_param(n, len, llen); // no trigger loop
       forall x | (AbLt(n, x) || n == x) && AbLt(x, s)
         ensures x in Elements(xs)
       {
-        if AbLt(x, AbAdd(n, llen)) {
+        if AbLt(x, AbInc(n, llen)) {
           SetEquality(Elements(L), bound);
         }
       }
     }
   } 
   else {
+    Props_inc_one (); Props_inc_zero (); // n + 1
     Props_int_pos(1); // 0 < 1
-    Props_two_is_one_plus_one ();
+    Props_all_nonneg ();
+    Props_lt2gteq (); // len < 2
+    Props_1inc1_is_2 ();
+    Props_inc_pos_is_lt ();
     Props_one_in_bound ();
-    Props_add_identity ();
-    Props_add_addition ();
-    Props_add_pos_is_neq (); // x + Positive != x
-    Props_add_is_leq (); // x + a == y ==> x < y || x == y
-    Props_add_pos_is_pos (); // x + Positive = Positive
   }
 }
 
@@ -359,27 +328,28 @@ function method SMN'(xs: List<AbInt>, n: AbInt, len: AbInt): AbInt
 {
   if xs == Nil then n
   else
-    var half := AbDiv2(AbAdd(len, int2adt(1))); // half = (len+1)/2
-    var (L, R) := Split(xs, AbAdd(n, half));
+    var half := AbDiv2(AbInc1(len)); // half = (len+1)/2
+    var (L, R) := Split(xs, AbInc(n, half));
     var llen := Length(L);
+
+    /* Props for ITE */
     Props_int_pos(1); // 0 < 1
-    Props_all_nonneg ();
-    // Props_add_identity ();
-    Props_add_pos_is_pos (); // x + Positive = Positive
-    Props_add_pos_is_lt (); // x < x + Positive
-    Props_gtzero_is_geqone_param (len); // x > 0 ==> x >= 1
-    Props_add_commutative ();
-    Props_lt_transitive ();
-    Props_div_add_leq_is_leq_param (len, int2adt(1));  // no trigger loop
+    Props_inc_one (); Props_inc_zero ();
+    Props_inc_pos_is_lt (); // x < x + Positive
+    Props_lt_transitive (); // len >= 1
+
     if AbLt(llen, half) then
+      Props_gt0_is_geq1 (); // x > 0 ==> x >= 1
+      Props_div_inc1_is_leq_param (len); // (x+1)/2 <= x
       Props_adt_dt_lt (llen, len);
       SMN'(L, n, llen)
     else
-      Props_add2sub ();
-      Props_lt_is_not_geq ();
-      Props_div_pos_is_pos ();
-      Props_adt_dt_lt (AbSub(len, llen), len);
-      SMN'(R, AbAdd(n, llen), AbSub(len, llen))
+      Props_all_nonneg ();
+      Props_lt2gteq ();
+      Props_div_pos ();
+      Props_inc2dec (); // llen is Positive
+      Props_adt_dt_lt (AbDec(len, llen), len);
+      SMN'(R, AbInc(n, llen), AbDec(len, llen))
 }
 
 lemma SMN'_Correct(xs: List<AbInt>, n: AbInt, len: AbInt)
@@ -388,47 +358,57 @@ lemma SMN'_Correct(xs: List<AbInt>, n: AbInt, len: AbInt)
   requires len == Length(xs)
   ensures var s := SMN'(xs, n, len);
     (AbLt(n, s) || n == s) &&
-    (AbLt(s, AbAdd(n, len)) || s == AbAdd(n, len)) &&
+    (AbLt(s, AbInc(n, len)) || s == AbInc(n, len)) &&
     s !in Elements(xs) &&
-    forall x ::(AbLt(n, x) || n == x) && AbLt(x, s) ==> x in Elements(xs)
+    forall x :: (AbLt(n, x) || n == x) && AbLt(x, s) ==> x in Elements(xs)
   decreases adt2dt(len)
 {
-  Props_lt_is_not_geq (); // x < y <==> !x > y && x != y
-  Props_add_identity ();
   if xs == Nil {
-  } else {
-    var half := AbDiv2(AbAdd(len, int2adt(1))); // half = (len+1)/2
-    var (L, R) := Split(xs, AbAdd(n, half));
-    Split_Correct(xs, AbAdd(n, half));
+    Props_inc_zero ();
+    Props_lt2gteq ();
+  } 
+  else {
+    var half := AbDiv2(AbInc1(len)); // half = (len+1)/2
+    var (L, R) := Split(xs, AbInc(n, half));
+    Split_Correct(xs, AbInc(n, half));
     var llen := Length(L);
     Elements_Property(L);  // use the NoDuplicates property
     var bound := IntRange(n, half);
     Cardinality(Elements(L), bound);
+    
+    /* Props for ITE */
     Props_int_pos(1); // 0 < 1
-    Props_all_nonneg ();
-    Props_add_pos_is_pos (); // x + Positive = Positive
-    Props_add_pos_is_lt (); // x < x + Positive
-    Props_gtzero_is_geqone_param (len); // x > 0 ==> x >= 1
-    Props_add_commutative ();
-    Props_lt_transitive ();
-    Props_div_add_leq_is_leq_param (len, int2adt(1));  // no trigger loop
+    Props_inc_one (); Props_inc_zero ();
+    Props_inc_pos_is_lt (); // x < x + Positive
+    Props_lt_transitive (); // len >= 1
+
     if AbLt(llen, half) {
       var s := SMN'(L, n, llen);
+      Props_gt0_is_geq1 (); // x > 0 ==> x >= 1
+      Props_div_inc1_is_leq_param (len);  // no trigger loop
       Props_adt_dt_lt (llen, len);
       SMN'_Correct(L, n, llen);
+
+      /* map boundary */
       Props_lt_addition ();
-      Props_add_less_is_lt_param(s, n, llen, len); // no trigger loop
-    } else {
-      Props_add2sub ();
-      Props_div_pos_is_pos ();
-      Props_adt_dt_lt (AbSub(len, llen), len);
-      var s := SMN'(R, AbAdd(n, llen), AbSub(len, llen));
-      SMN'_Correct(R, AbAdd(n, llen), AbSub(len, llen));
-      Props_add_sub_is_add_param(n, len, llen); // no trigger loop
+      Props_inc_lt_is_lt_param(s, n, llen, len); // no trigger loop
+    }
+    
+    else {
+      Props_all_nonneg ();
+      Props_lt2gteq ();
+      Props_div_pos ();
+      Props_inc2dec (); // llen is Positive
+      var s := SMN'(R, AbInc(n, llen), AbDec(len, llen));
+      Props_adt_dt_lt (AbDec(len, llen), len);
+      SMN'_Correct(R, AbInc(n, llen), AbDec(len, llen));
+
+      /* map boundary */
+      Props_inc_dec_is_inc_param(n, len, llen); // no trigger loop
       forall x | (AbLt(n, x) || n == x) && AbLt(x, s)
         ensures x in Elements(xs)
       {
-        if AbLt(x, AbAdd(n, llen)) {
+        if AbLt(x, AbInc(n, llen)) {
           SetEquality(Elements(L), bound);
         }
       }
@@ -442,29 +422,28 @@ function method SMN''(xs: List<AbInt>, n: AbInt, len: AbInt): AbInt
 {
   if xs == Nil then n
   else
-    var half := AbAdd(AbDiv2(len), int2adt(1)); // half = len/2 + 1
-    var (L, R) := Split(xs, AbAdd(n, half));
+    var half := AbInc1(AbDiv2(len)); // half = len/2 + 1
+    var (L, R) := Split(xs, AbInc(n, half));
     var llen := Length(L);
-    Props_int_pos(1); // 0 < 1
-    Props_all_nonneg ();
-    // Props_add_identity ();
-    Props_add_pos_is_pos (); // x + Positive = Positive
-    Props_add_pos_is_lt (); // x < x + Positive
-    Props_gtzero_is_geqone_param (len); // x > 0 ==> x >= 1
-    Props_add_commutative ();
+
+    /* Props for ITE */
+    Props_int_pos (1); // 0 < 1
+    Props_inc_one (); Props_inc_zero ();
+    Props_inc_pos_is_lt (); // x < x + Positive
     Props_lt_transitive ();
-    Props_div_addone_lt_param (len);
-    assert AbLt(half, len);
+
     if AbLt(llen, half) then
+      Props_gt0_is_geq1 (); // x > 0 ==> x >= 1
+      Props_div_and_inc1_is_leq_param (len); // x/2+1 <= x
       Props_adt_dt_lt (llen, len);
       SMN''(L, n, llen)
     else
-      Props_add2sub ();
-      Props_lt_is_not_geq ();
-      Props_div_pos_is_pos ();
-      Props_add_less_is_lt ();
-      Props_adt_dt_lt (AbSub(len, llen), len);
-      SMN''(R, AbAdd(n, llen), AbSub(len, llen))
+      Props_all_nonneg ();
+      Props_lt2gteq (); // llen >= len/2 + 1
+      Props_inc_pos_is_pos (); // 0 < x + 1
+      Props_inc2dec ();
+      Props_adt_dt_lt (AbDec(len, llen), len);
+      SMN''(R, AbInc(n, llen), AbDec(len, llen))
 }
 
 lemma SMN''_Correct(xs: List<AbInt>, n: AbInt, len: AbInt)
@@ -473,47 +452,55 @@ lemma SMN''_Correct(xs: List<AbInt>, n: AbInt, len: AbInt)
   requires len == Length(xs)
   ensures var s := SMN''(xs, n, len);
     (AbLt(n, s) || n == s) &&
-    (AbLt(s, AbAdd(n, len)) || s == AbAdd(n, len)) &&
+    (AbLt(s, AbInc(n, len)) || s == AbInc(n, len)) &&
     s !in Elements(xs) &&
-    forall x ::(AbLt(n, x) || n == x) && AbLt(x, s) ==> x in Elements(xs)
+    forall x :: (AbLt(n, x) || n == x) && AbLt(x, s) ==> x in Elements(xs)
   decreases adt2dt(len)
 {
-  Props_lt_is_not_geq (); // x < y <==> !x > y && x != y
-  Props_add_identity ();
   if xs == Nil {
-  } else {
-    var half := AbAdd(AbDiv2(len), int2adt(1)); // half = len/2 + 1
-    var (L, R) := Split(xs, AbAdd(n, half));
-    Split_Correct(xs, AbAdd(n, half));
+    Props_inc_zero ();
+    Props_lt2gteq ();
+  } 
+  else {
+    var half := AbInc1(AbDiv2(len)); // half = len/2 + 1
+    var (L, R) := Split(xs, AbInc(n, half));
+    Split_Correct(xs, AbInc(n, half));
     var llen := Length(L);
     Elements_Property(L);  // use the NoDuplicates property
     var bound := IntRange(n, half);
     Cardinality(Elements(L), bound);
-    Props_int_pos(1); // 0 < 1
-    Props_all_nonneg ();
-    Props_add_pos_is_pos (); // x + Positive = Positive
-    Props_add_pos_is_lt (); // x < x + Positive
-    Props_gtzero_is_geqone_param (len); // x > 0 ==> x >= 1
-    Props_add_commutative ();
+
+    /* Props for ITE */
+    Props_int_pos (1); // 0 < 1
+    Props_inc_one (); Props_inc_zero ();
+    Props_inc_pos_is_lt (); // x < x + Positive
     Props_lt_transitive ();
-    Props_div_addone_lt_param (len);
+
     if AbLt(llen, half) {
       var s := SMN''(L, n, llen);
+      Props_gt0_is_geq1 (); // x > 0 ==> x >= 1
+      Props_div_and_inc1_is_leq_param (len); // x/2+1 <= x
       Props_adt_dt_lt (llen, len);
       SMN''_Correct(L, n, llen);
+
+      /* map boundary */
       Props_lt_addition ();
-      Props_add_less_is_lt_param(s, n, llen, len); // no trigger loop
+      Props_inc_lt_is_lt_param(s, n, llen, len); // no trigger loop
     } else {
-      Props_add2sub ();
-      Props_div_pos_is_pos ();
-      Props_adt_dt_lt (AbSub(len, llen), len);
-      var s := SMN''(R, AbAdd(n, llen), AbSub(len, llen));
-      SMN''_Correct(R, AbAdd(n, llen), AbSub(len, llen));
-      Props_add_sub_is_add_param(n, len, llen); // no trigger loop
+      Props_all_nonneg ();
+      Props_lt2gteq (); // llen >= len/2 + 1
+      Props_inc_pos_is_pos (); // 0 < x + 1
+      Props_inc2dec ();
+      Props_adt_dt_lt (AbDec(len, llen), len);
+      var s := SMN''(R, AbInc(n, llen), AbDec(len, llen));
+      SMN''_Correct(R, AbInc(n, llen), AbDec(len, llen));
+
+      /* map boundary */
+      Props_inc_dec_is_inc_param(n, len, llen); // no trigger loop
       forall x | (AbLt(n, x) || n == x) && AbLt(x, s)
         ensures x in Elements(xs)
       {
-        if AbLt(x, AbAdd(n, llen)) {
+        if AbLt(x, AbInc(n, llen)) {
           SetEquality(Elements(L), bound);
         }
       }
@@ -521,32 +508,32 @@ lemma SMN''_Correct(xs: List<AbInt>, n: AbInt, len: AbInt)
   }
 }
 
-// TODO: need more concrete props to make it verified.
-method Main() {
-  var xs := Nil;
-  assert Length(xs) == int2adt(0);
-  var s := SmallestMissingNumber(xs);
-  Props_all_nonneg ();
-  Props_add_associative ();
-  Props_add_identity ();
-  Props_add_commutative ();
-  Props_add_pos_is_pos ();
-  Props_int_pos(2);
-  Props_lt_transitive ();
-  Props_lt_is_not_geq ();
-  assert s == int2adt(0);
-  print s, " ";  // 0
-  var a := Cons(int2adt(2), Cons(int2adt(0), Nil));
-  Props_two_is_one_plus_one ();
-  assume int2adt(1) == AbDiv2(int2adt(2));
-  assume AbLt(int2adt(0), int2adt(1));
-  assume AbLt(int2adt(1), int2adt(2));
-  // assert SmallestMissingNumbxer(a) == int2adt(1);
-  // print SmallestMissingNumber(a), " ";  // 1
-  a := Cons(int2adt(3), Cons(int2adt(1), a));
-  // assert SmallestMissingNumber(a) == int2adt(4);
-//   print SmallestMissingNumber(a), " ";  // 4
-  a := Cons(int2adt(7), Cons(int2adt(4), Cons(int2adt(6), a)));
-  // assert SmallestMissingNumber(a) == int2adt(5);
-//   print SmallestMissingNumber(a), "\n";  // 5
-}
+// // TODO: need more concrete props to make it verified.
+// method Main() {
+//   var xs := Nil;
+//   assert Length(xs) == int2adt(0);
+//   var s := SmallestMissingNumber(xs);
+//   Props_all_nonneg ();
+//   Props_inc_associative ();
+//   Props_add_identity ();
+//   Props_add_commutative ();
+//   Props_inc_pos ();
+//   Props_int_pos(2);
+//   Props_lt_transitive ();
+//   Props_lt2gteq ();
+//   assert s == int2adt(0);
+//   print s, " ";  // 0
+//   var a := Cons(int2adt(2), Cons(int2adt(0), Nil));
+//   Props_two_is_one_plus_one ();
+//   assume int2adt(1) == AbDiv2(int2adt(2));
+//   assume AbLt(int2adt(0), int2adt(1));
+//   assume AbLt(int2adt(1), int2adt(2));
+//   // assert SmallestMissingNumbxer(a) == int2adt(1);
+//   // print SmallestMissingNumber(a), " ";  // 1
+//   a := Cons(int2adt(3), Cons(int2adt(1), a));
+//   // assert SmallestMissingNumber(a) == int2adt(4);
+// //   print SmallestMissingNumber(a), " ";  // 4
+//   a := Cons(int2adt(7), Cons(int2adt(4), Cons(int2adt(6), a)));
+//   // assert SmallestMissingNumber(a) == int2adt(5);
+// //   print SmallestMissingNumber(a), "\n";  // 5
+// }
